Initialization file.

utils.v
@@ -1,7 +1,6 @@
 From Coq Require Import Program List.
-Set Universe Polymorphism.
 
-Set Implicit Arguments.
+Require Export init.
 
 (* Utilities *)
 
@@ -20,13 +19,13 @@ Inductive vec (A : Type) : nat -> Type :=
 
 (* induction scheme for vectors, taken from coq stdlib *)
 Definition rectS {A} (P : forall {n}, vec A (S n) -> Type)
-  (bas : forall a : A, P (vcons a (vnil _)))
+  (bas : forall a : A, P (vcons a vnil))
   (rect: forall a {n} (v : vec A (S n)), P v -> P (vcons a v)) :=
   fix rectS_fix {n} (v : vec A (S n)) : P v :=
   match v with
   |@vcons _ 0 a v =>
       match v with
-      | vnil _ => bas a
+      | vnil => bas a
       | _ => fun devil => False_ind (@IDProp) devil
       end
   |@vcons _ (S nn') a v => rect a v (rectS_fix v)
@@ -49,7 +48,7 @@ Definition vhd (A : Type) (n : nat) (v : vec A (S n)) : A :=
 Fixpoint quantify (A : Type) (n : nat)
   : (vec A n -> Type) -> Type :=
     match n return (vec A n -> Type) -> Type with
-    | O => fun f => f (vnil _)
+    | O => fun f => f vnil
     | S n' => fun f => forall a : A,
                 quantify (fun As => f (vcons a As))
     end.
@@ -59,13 +58,13 @@ Fixpoint curry (A : Type) (n : nat)
   : forall (G : vec A n -> Type), (forall X : vec A n, G X) -> quantify G :=
     match n return forall (G : vec A n -> Type),
     (forall X : vec A n, G X) -> quantify G with
-    | O => fun _ f => f (vnil _)
+    | O => fun _ f => f vnil
     | S n' => fun _ f => (fun a:A =>
                 curry _ (fun As => f (vcons a As)))
     end.
 
-Definition vec_nil_case {A : Type} (v : vec A 0) : v = vnil A :=
-  match v with (vnil _) => eq_refl end.
+Definition vec_nil_case {A : Type} (v : vec A 0) : v = vnil :=
+  match v with vnil => eq_refl end.
 
 Definition veq_hdtl {A : Type} {n : nat} (v : vec A (S n)) :
   v = vcons (vhd v) (vtl v).
@@ -87,30 +86,30 @@ Fixpoint uncurry' (n : nat) (A : Type) {struct n}
   : forall (G : vec A n -> Type), quantify G -> forall (va : vec A n), G va.
 Proof.
   intros G f va. induction n as [| n' IH].
-  - hnf in f. pose proof vec_nil_case va as H. rewrite H. exact f.
+  - hnf in f. pose proof vec_nil_case (v := va) as H. rewrite H. exact f.
   - hnf in f.
-    pose proof vec_cons_case va as H. destruct H as [a [As H]].
+    pose proof vec_cons_case (v := va) as H. destruct H as [a [As H]].
     rewrite H. exact (uncurry' _ _ _ (f a) As). Defined.
 
 (* uncurry a vector *)
 Fixpoint uncurryV (A B : Type) (n : nat) : nary_fn n A B -> vec A n -> B :=
   match n return nary_fn n A B -> vec A n -> B with
   | O => fun x _ => x
-  | S n' => fun f t => uncurryV _ (f (vhd t)) (vtl t)
+  | S n' => fun f t => uncurryV (f (vhd t)) (vtl t)
   end.
 
 (* apply a vector of functions to a vector *)
 Fixpoint zap (A B : Type) (n : nat) (vf : vec (A -> B) n)
   : vec A n -> vec B n :=
   match vf in vec _ n return vec _ n -> vec _ n with
-  | vnil _ => fun _ => vnil _
+  | vnil => fun _ => vnil
   | vcons f vf' => fun m => vcons (f (vhd m)) (zap vf' (vtl m))
   end.
 
 (* construct a vector with n elements of a:A *)
 Fixpoint repeat (n : nat) (A : Type) (a : A) : vec A n :=
   match n with
-  | O => vnil _
-  | S n' => vcons a (repeat _ a)
+  | O => vnil
+  | S n' => vcons a (repeat a)
   end.
 
