init.v
@@ -1,0 +1,6 @@
+Global Set Implicit Arguments.
+Global Set Strict Implicit.
+Global Set Strongly Strict Implicit.
+Global Set Contextual Implicit.
+Global Set Maximal Implicit Insertion.
+Global Set Universe Polymorphism.
